Make memappend spec a bit more readable
Todo: name subparts

src/program_proof/wal/heapspec.v
@@ -1480,23 +1480,33 @@ Proof.
     intro Hne. apply n. word.
 Qed.
 
+Definition memappend_crash_pre γh (bs: list update.t) (unmodifiedBlocks:  gmap u64 Block) crash_heaps γoldcrash : iProp Σ :=
+  ( [∗ map] a ↦ b ∈ unmodifiedBlocks, mapsto (hG := γoldcrash) a 1 b ) ∗
+  ⌜ ∀ u, u ∈ bs -> unmodifiedBlocks !! u.(update.addr) = None ⌝ ∗
+  own γh.(wal_heap_crash_heaps) (◯ Excl' crash_heaps).
+
+
+Definition memappend_crash γh (bs: list update.t) (unmodifiedBlocks:  gmap u64 Block)
+           crash_heaps γoldcrash pos lwh' new_crash_heap : iProp Σ :=
+  let γnewcrash := GenHeapG_Pre _ _ _ crashPreG new_crash_heap in
+     is_locked_walheap γh lwh' ∗
+     own γh.(wal_heap_crash_heaps) (◯ Excl' (async_put (pos, new_crash_heap) crash_heaps)) ∗
+    ( [∗ map] a ↦ b ∈ unmodifiedBlocks, mapsto (hG := γoldcrash) a 1 b ) ∗
+    ( [∗ map] a ↦ b ∈ unmodifiedBlocks, mapsto (hG := γnewcrash) a 1 b ) ∗
+    ( [∗ list] u ∈ bs, mapsto (hG := γnewcrash) u.(update.addr) 1 u.(update.b) ) ∗
+    txn_pos γh.(wal_heap_walnames) (length (possible crash_heaps)) pos.
+
+                                         
 Theorem wal_heap_memappend E γh bs (Q : u64 -> iProp Σ) lwh :
   ( |={⊤ ∖ ↑walN, E}=>
-          ∃ olds unmodifiedBlocks crash_heaps,
-            let γoldcrash := GenHeapG_Pre _ _ _ crashPreG (snd (latest crash_heaps)) in
-            memappend_pre γh.(wal_heap_h) bs olds ∗
-            ( [∗ map] a ↦ b ∈ unmodifiedBlocks, mapsto (hG := γoldcrash) a 1 b ) ∗
-            ⌜ ∀ u, u ∈ bs -> unmodifiedBlocks !! u.(update.addr) = None ⌝ ∗
-            own γh.(wal_heap_crash_heaps) (◯ Excl' crash_heaps) ∗
+      ∃ olds unmodifiedBlocks crash_heaps,
+        let γoldcrash := GenHeapG_Pre _ _ _ crashPreG (snd (latest crash_heaps)) in
+        memappend_pre γh.(wal_heap_h) bs olds ∗
+        memappend_crash_pre γh bs unmodifiedBlocks crash_heaps γoldcrash ∗
         ( ∀ pos lwh' new_crash_heap,
-          let γnewcrash := GenHeapG_Pre _ _ _ crashPreG new_crash_heap in
-          is_locked_walheap γh lwh' ∗
-          own γh.(wal_heap_crash_heaps) (◯ Excl' (async_put (pos, new_crash_heap) crash_heaps)) ∗
-          ( [∗ map] a ↦ b ∈ unmodifiedBlocks, mapsto (hG := γoldcrash) a 1 b ) ∗
-          ( [∗ map] a ↦ b ∈ unmodifiedBlocks, mapsto (hG := γnewcrash) a 1 b ) ∗
-          ( [∗ list] u ∈ bs, mapsto (hG := γnewcrash) u.(update.addr) 1 u.(update.b) ) ∗
-          txn_pos γh.(wal_heap_walnames) (length (possible crash_heaps)) pos ∗
-          memappend_q γh.(wal_heap_h) bs olds
+            memappend_crash γh bs unmodifiedBlocks crash_heaps γoldcrash pos lwh'
+                            new_crash_heap ∗
+            memappend_q γh.(wal_heap_h) bs olds
           ={E, ⊤ ∖ ↑walN}=∗ Q pos ) ) -∗
   is_locked_walheap γh lwh -∗
   ( ( ∀ σ σ' txn_id,
@@ -1515,7 +1525,9 @@ Proof using walheapG0.
   simpl in *; monad_inv.
   simpl in *.
 
-  iMod "Hpre" as (olds unmodifiedBlocks crash_heaps0) "(Hpre & Hunmodified & % & Hcrashheapsfrag & Hfupd)".
+  iMod "Hpre" as (olds unmodifiedBlocks crash_heaps0) "(Hpre & Hprecrash & Hfupd)".
+  iDestruct "Hprecrash" as "(Hunmodified & % & Hcrashheapsfrag)".
+
   iDestruct (ghost_var_agree with "Hcrash_heaps_own Hcrashheapsfrag") as "%"; subst.
   rename crash_heaps0 into crash_heaps.
 
@@ -1548,7 +1560,8 @@ Proof using walheapG0.
 
   iMod (ghost_var_update _ (async_put (pos', newcrashheap) crash_heaps) with "Hcrash_heaps_own Hcrashheapsfrag") as "[Hcrash_heaps_own Hcrashheapsfrag]".
 
-  iSpecialize ("Hfupd" $! (pos') (Build_locked_walheap _ _) newcrashheap).
+  iSpecialize ("Hfupd" $! (pos') (Build_locked_walheap _ _) newcrashheap ).
+
   iDestruct ("Hfupd" with "[$Hlockedheap $Hq $Hcrashheapsfrag $Hunmodified $Hunmodified_new $Hbs_new]") as "Hfupd".
   { admit. }
   iMod "Hfupd".
